Cpc/Proofs/RuleSupport/ResolutionSupport.lean
@@ -4544,8 +4544,7 @@ by
                             (Proof.pf (__eo_state_proven_nth s n2)) ≠ Term.Stuck at hProg
                           by_cases hPolTrue : pol = Term.Boolean true
                           · subst pol
-                            change StepRuleProperties M
-                              [__eo_state_proven_nth s n1, __eo_state_proven_nth s n2]
+                            change StepRuleProperties M [__eo_state_proven_nth s n1, __eo_state_proven_nth s n2]
                               (__eo_prog_resolution (Term.Boolean true) L
                                 (Proof.pf (__eo_state_proven_nth s n1))
                                 (Proof.pf (__eo_state_proven_nth s n2)))
@@ -4554,8 +4553,7 @@ by
                                 hC1Bool hC2Bool hProg
                           · by_cases hPolFalse : pol = Term.Boolean false
                             · subst pol
-                              change StepRuleProperties M
-                                [__eo_state_proven_nth s n1, __eo_state_proven_nth s n2]
+                              change StepRuleProperties M [__eo_state_proven_nth s n1, __eo_state_proven_nth s n2]
                                 (__eo_prog_resolution (Term.Boolean false) L
                                   (Proof.pf (__eo_state_proven_nth s n1))
                                   (Proof.pf (__eo_state_proven_nth s n2)))
